tests/demo/A_hpp_spec.v
@@ -7,7 +7,7 @@ Local Open Scope string_scope.
 From ChargeCore.Logics Require Import
      ILogic BILogic ILEmbed Later.
 
-Require Import Cpp.Auto. 
+Require Import Cpp.Auto.
 Require Demo.A_hpp.
 
 Definition A__foo := "_ZN1A3fooEi".
@@ -15,7 +15,7 @@ Definition A__foo_spec : function_spec' :=
   SFunction (Qmut T_int) (Qmut T_int :: nil)
       (fun x =>
          {| wpp_with := Z
-          ; wpp_pre := fun y => [| x = Vint y |] ** [| 0- 2^31 < (y + 6)%Z < 2^31 -1 |]
+          ; wpp_pre := fun y => [| x = Vint y |] ** [| has_type (y + 6) T_int |]
           ; wpp_post := fun y (r : val) => [| r = Vint (y + 6)%Z |]
           |}).
 
@@ -24,10 +24,10 @@ Definition A__bar_spec : function_spec' :=
   SFunction (Qmut T_int) (Qmut T_int :: nil)
       (fun x =>
          {| wpp_with := Z
-          ; wpp_pre := fun y => [| x = Vint y |] ** [| 0- 2^31 < (y + 7)%Z < 2^31 -1 |]
+          ; wpp_pre := fun y => [| x = Vint y |] ** [| has_type (y + 7) T_int |]
           ; wpp_post := fun y (r : val) => [| r = Vint (y + 7)%Z |]
           |}).
 
 Definition A_hpp_spec (resolve : _) :=
-      (|> Forall ti, cglob' (resolve:=resolve) A__foo ti A__foo_spec) -*
-          Forall ti, cglob' (resolve:=resolve) A__bar ti A__bar_spec.
+      (|> ti_cglob' (resolve:=resolve) A__foo A__foo_spec) -*
+          ti_cglob' (resolve:=resolve) A__bar A__bar_spec.
